compiler/regex/ManualProofsSSH.v
@@ -21,7 +21,7 @@ Definition SSH_TBL := (msg_d_authres, (msg_d_openpty, tt)).
 
 Record kstate_t {NB_MSG : nat} {PDV : payload_desc_vec NB_MSG} : Set := mkst_t
   { components : list fd
-    ; ktr : inhabited (Reflex.KTrace NB_MSG PDV)
+    ; ktr : inhabited (@KTrace NB_MSG PDV)
     ; system : fd
     ; slave : fd
     ; logincnt : num
@@ -37,8 +37,8 @@ Inductive ValidExchange :
     ValidExchange st
       (mkst_t _ _
          (components st)
-         (tr ~~~ KSend _ _ slv
-             (Build_msg SSH_NB_MSG SSH_TBL openpty_num
+         (tr ~~~ KSend slv
+             (@Build_msg SSH_NB_MSG SSH_TBL openpty_num
                         (username st, tt))::tr)
          (system st)
          (slave st)
@@ -50,8 +50,8 @@ Inductive ValidExchange :
    ValidExchange st
      (mkst_t _ _
         (components st)
-        (tr ~~~ KRecv _ _ sys
-            (Build_msg SSH_NB_MSG SSH_TBL authres_num
+        (tr ~~~ KRecv sys
+            (@Build_msg SSH_NB_MSG SSH_TBL authres_num
                        (user, (resnum, tt)))::tr)
         sys
         (slave st)
@@ -80,21 +80,21 @@ Definition RE_Auth_PTY user res : Regexp :=
     (RE_Star
        (RE_NAtom
           (@KOSend SSH_NB_MSG SSH_TBL None
-                  (@Build_opt_msg SSH_NB_MSG SSH_TBL
-                                  openpty_num
-                                  (Some user, tt)))))
+                  (Some (@Build_opt_msg SSH_NB_MSG SSH_TBL
+                                       openpty_num
+                                       (Some user, tt))))))
     (RE_Concat
        (RE_Star RE_Any)
        (RE_Concat (RE_Atom
                      (@KORecv SSH_NB_MSG SSH_TBL None
-                             (@Build_opt_msg SSH_NB_MSG SSH_TBL
-                                             authres_num
-                                             (Some user, (Some res, tt)))))
+                             (Some (@Build_opt_msg SSH_NB_MSG SSH_TBL
+                                                   authres_num
+                                                   (Some user, (Some res, tt))))))
                   (RE_NAtom
                      (@KOSend SSH_NB_MSG SSH_TBL None
-                             (@Build_opt_msg SSH_NB_MSG SSH_TBL
-                                             openpty_num
-                                             (Some user, tt)))))).
+                             (Some (@Build_opt_msg SSH_NB_MSG SSH_TBL
+                                                   openpty_num
+                                                   (Some user, tt))))))).
 
 
 (*This theorem is sort of cheating. It assumes that a successful response
@@ -103,3 +103,5 @@ Definition RE_Auth_PTY user res : Regexp :=
 Theorem priv_auth : forall st tr user,
   KInvariant st -> inhabits tr = ktr st ->
   RMatch (RE_Auth_PTY user (num_of_nat 1)) tr.
+Proof.
+  intros.
