compiler/regex/ReflexEcho.v
@@ -1,0 +1,45 @@
+Require Import String.
+
+Require Import Reflex.
+Require Import ReflexBase.
+Require Import ReflexDenoted.
+Require Import ReflexVec.
+Require Import Regex.
+Require Import Ynot.
+
+Definition NB_MSG : nat := 1.
+
+Definition PDV : payload_desc_vec NB_MSG :=
+  ( existT _ 1 (str_d, tt)
+  , tt
+  ).
+
+Definition HANDLERS : @handler NB_MSG PDV :=
+  (fun m =>
+    match tag m as _tm return
+      @sdenote _ SDenoted_payload_desc (@lkup_tag NB_MSG PDV _tm) -> _
+    with
+    | None => fun pl =>
+      let (s, _) := pl in
+         Send m (CurChan m) (MsgExpr m None (SLit m s, tt))
+      :: nil
+    | Some bad => fun _ =>
+      match bad with end
+    end (pay m)
+  )
+.
+
+Definition send_star NB_MSG PDV :=
+  RE_Star (RE_Alt (RE_Atom (@KOSend NB_MSG PDV None None))
+                  (RE_Atom (@KOExec NB_MSG PDV None None None))).
+
+Ltac unpack :=
+  match goal with
+  | [ H: [_]%inhabited = [_]%inhabited |- _ ] =>
+    apply pack_injective in H;
+    rewrite -> H in * || rewrite <- H in *
+  end.
+
+Theorem always_send : forall st tr,
+  Reach HANDLERS st -> inhabits tr = ktr st ->
+  RMatch (send_star NB_MSG PDV) tr.
